---
title: "GEKS_proofs"
author: "Matthew Stansfield"
date: "7/29/2020"
output: html_document
---

```{r setup, include=FALSE}
knitr::opts_chunk$set(echo = TRUE)
```

# Proofs for code

## Two important identities

The exponential of a sum is the product of the exponential of the summands.

$$a^{\sum_t^t x} = \prod_n^t a^{x}$$

Negative exponential

$$a^{-x} = 1/a^{x}$$
Where all $w_i(t,a) = 0$ and therefore $(p_i^a)^{w_i(\bullet,a)}$ is equal to 1

$$= \frac{(p_i^b)^{w_i(\bullet,b)}}{(p_i^a)^{w_i(\bullet,a)}}\cdot\left[\prod_t(p_i^t)^{\frac{(w_i(t,a)-w_i(t,b))}{T+1}}\right]$$

$$= \frac{(p_i^b)^{w_i(\bullet,b)}}{1}\cdot\left[\prod_t(p_i^t)^{\frac{0-w_i(t,b))}{T+1}}\right]$$


$$= \prod_t(p_i^b)^{\frac{w_i(t,b)}{T+1}}\cdot\left[\prod_t(\frac{1}{p_i^t})^{\frac{w_i(t,b)}{T+1}}\right]$$


$$= \prod_t(\frac{p_i^b}{p_i^t})^{\frac{w_i(t,b)}{T+1}}$$


Where all $w_i(t,b) = 0$ and therefore $(p_i^b)^{w_i(\bullet,b)}$ is equal to 1

$$= \frac{1}{(p_i^a)^{w_i(\bullet,a)}}\cdot\left[\prod_t(p_i^t)^{\frac{(w_i(t,a)-0)}{T+1}}\right]$$

$$= \frac{1}{\prod_t(p_i^a)^{\frac{w_i(t,a)}{T+1}}}\cdot\left[\prod_t(p_i^t)^{\frac{w_i(t,a)}{T+1}}\right]$$
Knowing $\frac{1}{\prod_i(x_i)}=\prod_i(\frac{1}{x_i})$

$$=\prod_t\frac{(p_i^t)^{\frac{w_i(t,a)}{T+1}}}{(p_i^a)^{\frac{w_i(t,a)}{T+1}}} $$

$$= \prod_t(\frac{p_i^t}{p_i^a})^{\frac{w_i(t,a)}{T+1}}$$